mergesort testing

TestTheories/Sorting.thy
@@ -20,12 +20,94 @@ fun isort :: "nat List \<Rightarrow> nat List" where
 
 fun qsort :: "nat list \<Rightarrow> nat list" where
   "qsort [] = []"
-| "qsort (t # ts) = [r . r <- ts, r \<le> t] @ (t # [r . r <- ts, \<not> (r \<le> t)])"
+| "qsort (t # ts) = (qsort [r <- ts. r \<le> t]) @ [t] @ (qsort [r <- ts. \<not> (r \<le> t)])"
+
 
 fun sorted' :: "nat list \<Rightarrow> bool" where
   "sorted' []                   = True"
 | "sorted' [x]         = True"
-| "sorted' (r # (t # ts))  = (r \<le> t \<and>  sorted' (t # ts))"
+| "sorted' (r # (t # ts))  = (r \<le> t \<and> sorted' (t # ts))"
+
+fun merge :: "nat list \<Rightarrow> nat list \<Rightarrow> nat list" where
+  "merge rs [] = rs"
+| "merge [] ts = ts"
+| "merge (r#rs) (t#ts) = (if r \<le> t then r # merge rs (t#ts) else t # merge (r#rs) ts)"
+
+fun msort :: "nat list => nat list" where
+  "msort [] = []"
+| "msort [t] = [t]"
+| "msort ts = merge (msort (List.take (length ts div 2) ts)) (* size instead? *)
+                    (msort (List.drop (length ts div 2) ts))"
+
+lemma sortCons: "r \<le> t \<and> sorted' (t # ts) \<Longrightarrow> sorted' (r # (t # ts))"
+by simp
+
+lemma mer1: "sorted' ts \<Longrightarrow> sorted' (merge [] ts)"
+(*by(metis sorted'.cases merge.simps)*) (* replace of cases by inductions *)
+by hipster_induct_simp_metis
+
+lemma mer2: "sorted' ts \<Longrightarrow> sorted' (merge [t] ts)" (* sorted'.induct! *)
+by hipster_induct_schemes
+
+lemma mer3: "sorted' ts \<Longrightarrow> sorted' (merge ts [t])" (* sorted'.induct! *)
+by hipster_induct_schemes
+
+lemma mer4: "sorted' (t # ts) \<and> \<not> t \<le> r \<Longrightarrow> sorted' (r # (merge (t#ts) []))"
+by simp
+
+lemma mer4': "sorted' (t # ts) \<and> t \<le> r \<Longrightarrow> sorted' (t # merge ts [r])"
+by (hipster_induct_schemes merge.simps mer3)
+
+lemma mer5': "sorted' (t # ts) \<and> r \<le> v \<and> \<not> t \<le> r \<Longrightarrow> sorted' (r # (merge (t#ts) [v]))"
+(*apply(induction ts rule: sorted'.induct)
+apply(simp_all add: mer4 mer3 mer2 mer1)
+apply(metis sorted'.simps merge.simps)*)
+by (hipster_induct_schemes merge.simps mer3)
+
+lemma mer5'': "sorted' (r # rs) \<and> \<not> t \<le> r \<Longrightarrow> sorted' (r # (merge [t] rs))"
+by (hipster_induct_schemes sorted'.simps)
+
+(*lemma merComm: "sorted' ts \<and> sorted' rs \<Longrightarrow> merge rs ts = merge ts rs"
+apply(induction rs ts rule: merge.induct)
+apply(simp_all)
+apply(metis sorted'.cases merge.simps(1) merge.simps(2))*)
+
+(* simplification can very much screw up the goal state! *)
+lemma mer5: "(sorted' (t # ts) \<and> sorted' (r # rs) \<and> t \<le> r) \<Longrightarrow> (sorted' (t # (merge ts (r#rs))))"
+apply(induction ts rule: sorted'.induct)
+apply(simp)
+apply(simp add: mer5'')
+apply(simp add: mer5' mer4') (*
+apply(metis merge.simps(3) mer5' mer4' mer3 mer4)*)
+sorry
+
+lemma cons1: "sorted' (t # ts) \<Longrightarrow> sorted' ts"
+by hipster_induct_simp_metis
+(*by (metis sorted'.elims(3) sorted'.simps(3))*)
+
+lemma mergeS: "sorted' ts \<and> sorted' rs \<Longrightarrow> sorted' (merge ts rs)"
+(* apply(induction ts rs rule: merge.induct)
+apply(simp_all add: mer1 mer2)
+by (metis mer4 mer5 merge.simps sorted'.simps)*)
+apply(cases rs)
+apply(simp_all)
+by (hipster_induct_schemes mer1 mer5'' mer5 merge.simps sorted'.simps)
+(*apply(induction ts rule: sorted'.induct)
+apply(simp add: mer1)
+apply(simp add: mer5'')
+by (metis mer4 mer5 merge.simps sorted'.simps)*)
+(* apply(induction ts rule: sorted'.induct)
+apply(simp add: mer1)
+apply(simp add: mer2)
+apply(cases rs)
+apply(simp_all)
+by (metis mer4 mer5 merge.simps sorted'.simps)*)
+(*   by (induct xs ys rule: merge.induct) (auto simp add: ball_Un not_le less_le sorted_Cons) *)
+
+lemma smsort: "sorted' (msort xs)"
+by (hipster_induct_schemes mergeS)
+
+
 
 (*
 fun merge :: "Nat list \<Rightarrow> Nat list \<Rightarrow> Nat list" where
